07TailCall/TailCallOptimization.thy
@@ -2,26 +2,26 @@ theory TailCallOptimization
   imports TailCall "../06TreeCode/TreeCode" "../00Utils/Iteration"
 begin
 
-fun tco_r :: "tree_code list \<Rightarrow> tco_return" where
+fun tco_r :: "code\<^sub>e list \<Rightarrow> tco_return" where
   "tco_r [] = TCOReturn"
-| "tco_r (TApply # cd) = (case cd of [] \<Rightarrow> TCOJump | _ \<Rightarrow> tco_r cd)"
+| "tco_r (Apply\<^sub>e # cd) = (case cd of [] \<Rightarrow> TCOJump | _ \<Rightarrow> tco_r cd)"
 | "tco_r (op # cd) = tco_r cd"
 
-fun tco_cd :: "tree_code list \<Rightarrow> tco_code list" where
+fun tco_cd :: "code\<^sub>e list \<Rightarrow> tco_code list" where
   "tco_cd [] = []"
-| "tco_cd (TLookup x # cd) = TCOLookup x # tco_cd cd"
-| "tco_cd (TPushCon k # cd) = TCOPushCon k # tco_cd cd"
-| "tco_cd (TPushLam cd' # cd) = TCOPushLam (tco_cd cd') (tco_r cd') # tco_cd cd"
-| "tco_cd (TApply # cd) = (case cd of [] \<Rightarrow> [] | _ \<Rightarrow> TCOApply # tco_cd cd)"
+| "tco_cd (Lookup\<^sub>e x # cd) = TCOLookup x # tco_cd cd"
+| "tco_cd (PushCon\<^sub>e k # cd) = TCOPushCon k # tco_cd cd"
+| "tco_cd (PushLam\<^sub>e cd' # cd) = TCOPushLam (tco_cd cd') (tco_r cd') # tco_cd cd"
+| "tco_cd (Apply\<^sub>e # cd) = (case cd of [] \<Rightarrow> [] | _ \<Rightarrow> TCOApply # tco_cd cd)"
 
-definition tco :: "tree_code list \<Rightarrow> tco_code list \<times> tco_return" where
+definition tco :: "code\<^sub>e list \<Rightarrow> tco_code list \<times> tco_return" where
   "tco cd = (tco_cd cd, tco_r cd)"
 
-primrec tco_val :: "tclosure \<Rightarrow> tco_closure" where
-  "tco_val (TConst k) = TCOConst k"
-| "tco_val (TLam vs cd) = TCOLam (map tco_val vs) (tco_cd cd) (tco_r cd)"
+primrec tco_val :: "closure\<^sub>e \<Rightarrow> tco_closure" where
+  "tco_val (Const\<^sub>e k) = TCOConst k"
+| "tco_val (Lam\<^sub>e vs cd) = TCOLam (map tco_val vs) (tco_cd cd) (tco_r cd)"
 
-fun tco_stack_frame :: "tree_stack_frame \<Rightarrow> tco_stack_frame" where
+fun tco_stack_frame :: "frame\<^sub>e \<Rightarrow> tco_stack_frame" where
   "tco_stack_frame (vs, cd) = (map tco_val vs, tco_cd cd, tco_r cd)"
 
 fun live_frame :: "tco_stack_frame \<Rightarrow> bool" where
@@ -29,14 +29,14 @@ fun live_frame :: "tco_stack_frame \<Rightarrow> bool" where
 | "live_frame (vs, [], TCOJump) = True"
 | "live_frame (vs, op # cd, r) = True"
 
-primrec dead_frame :: "tree_stack_frame \<Rightarrow> bool" where
+primrec dead_frame :: "frame\<^sub>e \<Rightarrow> bool" where
   "dead_frame (vs, cd) = (cd = [])"
 
-abbreviation tco_stack :: "tree_stack_frame list \<Rightarrow> tco_stack_frame list" where
+abbreviation tco_stack :: "frame\<^sub>e list \<Rightarrow> tco_stack_frame list" where
   "tco_stack sfs \<equiv> filter live_frame (map tco_stack_frame sfs)"
 
-primrec tco_state :: "tree_code_state \<Rightarrow> tco_code_state" where
-  "tco_state (TS vs sfs) = TCOS (map tco_val vs) (tco_stack sfs)"
+primrec tco_state :: "state\<^sub>e \<Rightarrow> tco_code_state" where
+  "tco_state (S\<^sub>e vs sfs) = TCOS (map tco_val vs) (tco_stack sfs)"
 
 lemma [simp]: "cd \<noteq> [] \<Longrightarrow> tco_r (op # cd) = tco_r cd"
   by (induction op) (simp_all split: list.splits)
@@ -101,49 +101,49 @@ proof (induction sfs')
 qed simp_all
 
 lemma [dest]: "TCOS vs ((env, cd, r) # sfs) = tco_state \<Sigma> \<Longrightarrow> \<exists>dsfs vs' env' cd' sfs'. 
-  \<Sigma> = TS vs' (dsfs @ (env', cd') # sfs') \<and> vs = map tco_val vs' \<and> env = map tco_val env' \<and> 
+  \<Sigma> = S\<^sub>e vs' (dsfs @ (env', cd') # sfs') \<and> vs = map tco_val vs' \<and> env = map tco_val env' \<and> 
     cd = tco_cd cd' \<and> r = tco_r cd' \<and> list_all dead_frame dsfs \<and> sfs = tco_stack sfs'"
   by (induction \<Sigma>) auto
 
-lemma [dest]: "TCOLookup x # cd = tco_cd cd' \<Longrightarrow> \<exists>cd''. cd' = TLookup x # cd'' \<and> cd = tco_cd cd''"
+lemma [dest]: "TCOLookup x # cd = tco_cd cd' \<Longrightarrow> \<exists>cd''. cd' = Lookup\<^sub>e x # cd'' \<and> cd = tco_cd cd''"
   by (induction cd' rule: tco_cd.induct) (simp_all split: list.splits)
 
-lemma [dest]: "TCOPushCon k # cd = tco_cd cd' \<Longrightarrow> \<exists>cd''. cd' = TPushCon k # cd'' \<and> cd = tco_cd cd''"
+lemma [dest]: "TCOPushCon k # cd = tco_cd cd' \<Longrightarrow> \<exists>cd''. cd' = PushCon\<^sub>e k # cd'' \<and> cd = tco_cd cd''"
   by (induction cd' rule: tco_cd.induct) (simp_all split: list.splits)
 
-lemma [dest]: "TCOPushLam cd' r # cd = tco_cd cd\<^sub>t \<Longrightarrow> \<exists>cd\<^sub>t' cd\<^sub>t''. cd\<^sub>t = TPushLam cd\<^sub>t'' # cd\<^sub>t' \<and> 
+lemma [dest]: "TCOPushLam cd' r # cd = tco_cd cd\<^sub>t \<Longrightarrow> \<exists>cd\<^sub>t' cd\<^sub>t''. cd\<^sub>t = PushLam\<^sub>e cd\<^sub>t'' # cd\<^sub>t' \<and> 
     cd = tco_cd cd\<^sub>t' \<and> r = tco_r cd\<^sub>t'' \<and> cd' = tco_cd cd\<^sub>t''"
   by (induction cd\<^sub>t rule: tco_cd.induct) (simp_all split: list.splits)
 
 lemma [dest]: "TCOApply # cd = tco_cd cd' \<Longrightarrow> 
-    \<exists>op cd''. cd' = TApply # op # cd'' \<and> cd = tco_cd (op # cd'')"
+    \<exists>op cd''. cd' = Apply\<^sub>e # op # cd'' \<and> cd = tco_cd (op # cd'')"
   by (induction cd' rule: tco_cd.induct) (simp_all split: list.splits)
 
-lemma [dest]: "TCOConst k = tco_val v \<Longrightarrow> v = TConst k"
+lemma [dest]: "TCOConst k = tco_val v \<Longrightarrow> v = Const\<^sub>e k"
   by (induction v) simp_all
 
 lemma [dest]: "TCOLam env cd r = tco_val v \<Longrightarrow> 
-    \<exists>env\<^sub>t cd\<^sub>t. v = TLam env\<^sub>t cd\<^sub>t \<and> env = map tco_val env\<^sub>t \<and> cd = tco_cd cd\<^sub>t \<and> r = tco_r cd\<^sub>t"
+    \<exists>env\<^sub>t cd\<^sub>t. v = Lam\<^sub>e env\<^sub>t cd\<^sub>t \<and> env = map tco_val env\<^sub>t \<and> cd = tco_cd cd\<^sub>t \<and> r = tco_r cd\<^sub>t"
   by (induction v) simp_all
 
 lemma [dest]: "TCOReturn = tco_r cd \<Longrightarrow> [] = tco_cd cd \<Longrightarrow> cd = []"
   by (induction cd rule: tco_cd.induct) (simp_all split: list.splits)
 
-lemma [dest]: "TCOJump = tco_r cd \<Longrightarrow> [] = tco_cd cd \<Longrightarrow> cd = [TApply]"
+lemma [dest]: "TCOJump = tco_r cd \<Longrightarrow> [] = tco_cd cd \<Longrightarrow> cd = [Apply\<^sub>e]"
   by (induction cd rule: tco_cd.induct) (simp_all split: list.splits)
 
-lemma [simp]: "list_all dead_frame dsfs \<Longrightarrow> iter (\<leadsto>\<^sub>t) (TS vs (dsfs @ sfs)) (TS vs sfs)"
+lemma [simp]: "list_all dead_frame dsfs \<Longrightarrow> iter (\<leadsto>\<^sub>e) (S\<^sub>e vs (dsfs @ sfs)) (S\<^sub>e vs sfs)"
 proof (induction dsfs)
   case (Cons sf dsfs)
   then obtain vs' where "sf = (vs', [])" by (cases sf) simp_all
-  hence "TS vs ((sf # dsfs) @ sfs) \<leadsto>\<^sub>t TS vs (dsfs @ sfs)" by simp
+  hence "S\<^sub>e vs ((sf # dsfs) @ sfs) \<leadsto>\<^sub>e S\<^sub>e vs (dsfs @ sfs)" by simp
   with Cons show ?case by simp
 qed simp_all
 
-lemma [simp]: "\<not> live_frame fr \<Longrightarrow> iter (\<leadsto>\<^sub>t\<^sub>c\<^sub>o) (TCOS vs (fr # sfs)) (TCOS vs sfs)"
+lemma [simp]: "\<not> live_frame fr \<Longrightarrow> iter (\<leadsto>\<^sub>e\<^sub>c\<^sub>o) (TCOS vs (fr # sfs)) (TCOS vs sfs)"
 proof (induction fr rule: live_frame.induct)
   case (1 env)
-  hence "TCOS vs ((env, [], TCOReturn) # sfs) \<leadsto>\<^sub>t\<^sub>c\<^sub>o TCOS vs sfs" by simp
+  hence "TCOS vs ((env, [], TCOReturn) # sfs) \<leadsto>\<^sub>e\<^sub>c\<^sub>o TCOS vs sfs" by simp
   thus ?case by (metis iter_one)
 qed simp_all
 
@@ -156,190 +156,187 @@ lemma [simp]: "live_frame (env, cd, TCOJump)"
 lemma tco_never_dead [simp]: "live_frame (env, tco_cd (op # cd), tco_r (op # cd))"
   by (induction op) (simp_all split: list.splits)
 
-theorem completetco [simp]: "tco_state \<Sigma>\<^sub>t \<leadsto>\<^sub>t\<^sub>c\<^sub>o \<Sigma>' \<Longrightarrow> full_state \<Sigma>\<^sub>t \<Longrightarrow> \<exists>\<Sigma>\<^sub>t'. iter (\<leadsto>\<^sub>t) \<Sigma>\<^sub>t \<Sigma>\<^sub>t' \<and> 
-  iter (\<leadsto>\<^sub>t\<^sub>c\<^sub>o) \<Sigma>' (tco_state \<Sigma>\<^sub>t')"
+theorem completetco [simp]: "tco_state \<Sigma>\<^sub>t \<leadsto>\<^sub>e\<^sub>c\<^sub>o \<Sigma>' \<Longrightarrow> \<exists>\<Sigma>\<^sub>t'. iter (\<leadsto>\<^sub>e) \<Sigma>\<^sub>t \<Sigma>\<^sub>t' \<and> 
+  iter (\<leadsto>\<^sub>e\<^sub>c\<^sub>o) \<Sigma>' (tco_state \<Sigma>\<^sub>t')"
 proof (induction "tco_state \<Sigma>\<^sub>t" \<Sigma>' rule: evaltco.induct)
   case (evtco_lookup env x v vs cd r sfs)
   then obtain dsfs vs' env' cd' sfs' where S: 
-    "\<Sigma>\<^sub>t = TS vs' (dsfs @ (env', TLookup x # cd') # sfs') \<and> vs = map tco_val vs' \<and> 
+    "\<Sigma>\<^sub>t = S\<^sub>e vs' (dsfs @ (env', Lookup\<^sub>e x # cd') # sfs') \<and> vs = map tco_val vs' \<and> 
       env = map tco_val env' \<and> cd = tco_cd cd' \<and> r = tco_r cd' \<and> list_all dead_frame dsfs \<and> 
         sfs = tco_stack sfs'" by fastforce
   with evtco_lookup obtain v' where V: "lookup env' x = Some v' \<and> v = tco_val v'" by fastforce
-  from S have "iter (\<leadsto>\<^sub>t) (TS vs' (dsfs @ (env', TLookup x # cd') # sfs')) 
-    (TS vs' ((env', TLookup x # cd') # sfs'))" by simp
-  moreover from V have "iter (\<leadsto>\<^sub>t) (TS vs' ((env', TLookup x # cd') # sfs')) 
-    (TS (v' # vs') ((env', cd') # sfs'))" by (metis evt_lookup iter_one)
-  ultimately have X: "iter (\<leadsto>\<^sub>t) (TS vs' (dsfs @ (env', TLookup x # cd') # sfs')) 
-    (TS (v' # vs') ((env', cd') # sfs'))" by (metis iter_append)
-  from S V have "iter (\<leadsto>\<^sub>t\<^sub>c\<^sub>o) (TCOS (v # map tco_val vs') 
+  from S have "iter (\<leadsto>\<^sub>e) (S\<^sub>e vs' (dsfs @ (env', Lookup\<^sub>e x # cd') # sfs')) 
+    (S\<^sub>e vs' ((env', Lookup\<^sub>e x # cd') # sfs'))" by simp
+  moreover from V have "iter (\<leadsto>\<^sub>e) (S\<^sub>e vs' ((env', Lookup\<^sub>e x # cd') # sfs')) 
+    (S\<^sub>e (v' # vs') ((env', cd') # sfs'))" by (metis ev\<^sub>e_lookup iter_one)
+  ultimately have X: "iter (\<leadsto>\<^sub>e) (S\<^sub>e vs' (dsfs @ (env', Lookup\<^sub>e x # cd') # sfs')) 
+    (S\<^sub>e (v' # vs') ((env', cd') # sfs'))" by (metis iter_append)
+  from S V have "iter (\<leadsto>\<^sub>e\<^sub>c\<^sub>o) (TCOS (v # map tco_val vs') 
     ((map tco_val env', tco_cd cd', tco_r cd') # tco_stack sfs')) 
-      (tco_state (TS (v' # vs') ((env', cd') # sfs')))" by simp
+      (tco_state (S\<^sub>e (v' # vs') ((env', cd') # sfs')))" by simp
   with S X show ?case by blast
 next
   case (evtco_pushcon vs env k cd r sfs)
   then obtain dsfs vs' env' cd' sfs' where S: 
-    "\<Sigma>\<^sub>t = TS vs' (dsfs @ (env', TPushCon k # cd') # sfs') \<and> vs = map tco_val vs' \<and> 
+    "\<Sigma>\<^sub>t = S\<^sub>e vs' (dsfs @ (env', PushCon\<^sub>e k # cd') # sfs') \<and> vs = map tco_val vs' \<and> 
       env = map tco_val env' \<and> cd = tco_cd cd' \<and> r = tco_r cd' \<and> list_all dead_frame dsfs \<and> 
         sfs = tco_stack sfs'" by fastforce
-  hence "iter (\<leadsto>\<^sub>t) (TS vs' (dsfs @ (env', TPushCon k # cd') # sfs')) 
-    (TS vs' ((env', TPushCon k # cd') # sfs'))" by simp
-  moreover have "iter (\<leadsto>\<^sub>t) (TS vs' ((env', TPushCon k # cd') # sfs')) 
-    (TS (TConst k # vs') ((env', cd') # sfs'))" by (metis evt_pushcon iter_one)
-  ultimately have X: "iter (\<leadsto>\<^sub>t) (TS vs' (dsfs @ (env', TPushCon k # cd') # sfs')) 
-    (TS (TConst k # vs') ((env', cd') # sfs'))" by simp
-  from S have "iter (\<leadsto>\<^sub>t\<^sub>c\<^sub>o) (TCOS (TCOConst k # map tco_val vs') 
+  hence "iter (\<leadsto>\<^sub>e) (S\<^sub>e vs' (dsfs @ (env', PushCon\<^sub>e k # cd') # sfs')) 
+    (S\<^sub>e vs' ((env', PushCon\<^sub>e k # cd') # sfs'))" by simp
+  moreover have "iter (\<leadsto>\<^sub>e) (S\<^sub>e vs' ((env', PushCon\<^sub>e k # cd') # sfs')) 
+    (S\<^sub>e (Const\<^sub>e k # vs') ((env', cd') # sfs'))" by (metis ev\<^sub>e_pushcon iter_one)
+  ultimately have X: "iter (\<leadsto>\<^sub>e) (S\<^sub>e vs' (dsfs @ (env', PushCon\<^sub>e k # cd') # sfs')) 
+    (S\<^sub>e (Const\<^sub>e k # vs') ((env', cd') # sfs'))" by simp
+  from S have "iter (\<leadsto>\<^sub>e\<^sub>c\<^sub>o) (TCOS (TCOConst k # map tco_val vs') 
     ((map tco_val env', tco_cd cd', tco_r cd') # tco_stack sfs')) 
-      (tco_state (TS (TConst k # vs') ((env', cd') # sfs')))" by simp
+      (tco_state (S\<^sub>e (Const\<^sub>e k # vs') ((env', cd') # sfs')))" by simp
   with S X show ?case by blast
 next
   case (evtco_pushlam vs env cd' r' cd r sfs)
   then obtain dsfs vs\<^sub>t env\<^sub>t cd\<^sub>t cd\<^sub>t' sfs\<^sub>t where S: 
-    "\<Sigma>\<^sub>t = TS vs\<^sub>t (dsfs @ (env\<^sub>t, TPushLam cd\<^sub>t' # cd\<^sub>t) # sfs\<^sub>t) \<and> vs = map tco_val vs\<^sub>t \<and> 
+    "\<Sigma>\<^sub>t = S\<^sub>e vs\<^sub>t (dsfs @ (env\<^sub>t, PushLam\<^sub>e cd\<^sub>t' # cd\<^sub>t) # sfs\<^sub>t) \<and> vs = map tco_val vs\<^sub>t \<and> 
       env = map tco_val env\<^sub>t \<and> cd = tco_cd cd\<^sub>t \<and> cd' = tco_cd cd\<^sub>t' \<and> r' = tco_r cd\<^sub>t' \<and> 
         r = tco_r cd\<^sub>t \<and> list_all dead_frame dsfs \<and> sfs = tco_stack sfs\<^sub>t" by fastforce
-  hence "iter (\<leadsto>\<^sub>t) (TS vs\<^sub>t (dsfs @ (env\<^sub>t, TPushLam cd\<^sub>t' # cd\<^sub>t) # sfs\<^sub>t)) 
-    (TS vs\<^sub>t ((env\<^sub>t, TPushLam cd\<^sub>t' # cd\<^sub>t) # sfs\<^sub>t))" by simp
-  moreover have "iter (\<leadsto>\<^sub>t) (TS vs\<^sub>t ((env\<^sub>t, TPushLam cd\<^sub>t' # cd\<^sub>t) # sfs\<^sub>t)) 
-    (TS (TLam env\<^sub>t cd\<^sub>t' # vs\<^sub>t) ((env\<^sub>t, cd\<^sub>t) # sfs\<^sub>t))" by (metis evt_pushlam iter_one)
-  ultimately have X: "iter (\<leadsto>\<^sub>t) (TS vs\<^sub>t (dsfs @ (env\<^sub>t, TPushLam cd\<^sub>t' # cd\<^sub>t) # sfs\<^sub>t)) 
-    (TS (TLam env\<^sub>t cd\<^sub>t' # vs\<^sub>t) ((env\<^sub>t, cd\<^sub>t) # sfs\<^sub>t))" by simp
-  from S have "iter (\<leadsto>\<^sub>t\<^sub>c\<^sub>o) (TCOS (TCOLam env cd' r' # map tco_val vs\<^sub>t) 
+  hence "iter (\<leadsto>\<^sub>e) (S\<^sub>e vs\<^sub>t (dsfs @ (env\<^sub>t, PushLam\<^sub>e cd\<^sub>t' # cd\<^sub>t) # sfs\<^sub>t)) 
+    (S\<^sub>e vs\<^sub>t ((env\<^sub>t, PushLam\<^sub>e cd\<^sub>t' # cd\<^sub>t) # sfs\<^sub>t))" by simp
+  moreover have "iter (\<leadsto>\<^sub>e) (S\<^sub>e vs\<^sub>t ((env\<^sub>t, PushLam\<^sub>e cd\<^sub>t' # cd\<^sub>t) # sfs\<^sub>t)) 
+    (S\<^sub>e (Lam\<^sub>e env\<^sub>t cd\<^sub>t' # vs\<^sub>t) ((env\<^sub>t, cd\<^sub>t) # sfs\<^sub>t))" by (metis ev\<^sub>e_pushlam iter_one)
+  ultimately have X: "iter (\<leadsto>\<^sub>e) (S\<^sub>e vs\<^sub>t (dsfs @ (env\<^sub>t, PushLam\<^sub>e cd\<^sub>t' # cd\<^sub>t) # sfs\<^sub>t)) 
+    (S\<^sub>e (Lam\<^sub>e env\<^sub>t cd\<^sub>t' # vs\<^sub>t) ((env\<^sub>t, cd\<^sub>t) # sfs\<^sub>t))" by simp
+  from S have "iter (\<leadsto>\<^sub>e\<^sub>c\<^sub>o) (TCOS (TCOLam env cd' r' # map tco_val vs\<^sub>t) 
     ((map tco_val env\<^sub>t, tco_cd cd\<^sub>t, tco_r cd\<^sub>t) # tco_stack sfs\<^sub>t)) 
-      (tco_state (TS (TLam env\<^sub>t cd\<^sub>t' # vs\<^sub>t) ((env\<^sub>t, cd\<^sub>t) # sfs\<^sub>t)))" by simp
+      (tco_state (S\<^sub>e (Lam\<^sub>e env\<^sub>t cd\<^sub>t' # vs\<^sub>t) ((env\<^sub>t, cd\<^sub>t) # sfs\<^sub>t)))" by simp
   with S X show ?case by blast
 next
   case (evtco_apply v env' cd' r' vs env cd r sfs)
   then obtain dsfs v\<^sub>t vl vs\<^sub>t env\<^sub>t cd\<^sub>t'' sfs\<^sub>t where S: 
-    "\<Sigma>\<^sub>t = TS (v\<^sub>t # vl # vs\<^sub>t) (dsfs @ (env\<^sub>t, cd\<^sub>t'') # sfs\<^sub>t) \<and> v = tco_val v\<^sub>t \<and> 
+    "\<Sigma>\<^sub>t = S\<^sub>e (v\<^sub>t # vl # vs\<^sub>t) (dsfs @ (env\<^sub>t, cd\<^sub>t'') # sfs\<^sub>t) \<and> v = tco_val v\<^sub>t \<and> 
       TCOLam env' cd' r' = tco_val vl \<and> vs = map tco_val vs\<^sub>t \<and> env = map tco_val env\<^sub>t \<and> 
         TCOApply # cd = tco_cd cd\<^sub>t'' \<and> r = tco_r cd\<^sub>t'' \<and> list_all dead_frame dsfs \<and> 
           sfs = tco_stack sfs\<^sub>t" by blast
-  then obtain op cd\<^sub>t where C: "cd\<^sub>t'' = TApply # op # cd\<^sub>t \<and> cd = tco_cd (op # cd\<^sub>t)" by blast
-  from S obtain env\<^sub>t' cd\<^sub>t' where V: "vl = TLam env\<^sub>t' cd\<^sub>t' \<and> env' = map tco_val env\<^sub>t' \<and> 
+  then obtain op cd\<^sub>t where C: "cd\<^sub>t'' = Apply\<^sub>e # op # cd\<^sub>t \<and> cd = tco_cd (op # cd\<^sub>t)" by blast
+  from S obtain env\<^sub>t' cd\<^sub>t' where V: "vl = Lam\<^sub>e env\<^sub>t' cd\<^sub>t' \<and> env' = map tco_val env\<^sub>t' \<and> 
     cd' = tco_cd cd\<^sub>t' \<and> r' = tco_r cd\<^sub>t'" by blast
-  from S have "iter (\<leadsto>\<^sub>t) (TS (v\<^sub>t # TLam env\<^sub>t' cd\<^sub>t' # vs\<^sub>t) (dsfs @ (env\<^sub>t, TApply # op # cd\<^sub>t) # sfs\<^sub>t)) 
-    (TS (v\<^sub>t # TLam env\<^sub>t' cd\<^sub>t' # vs\<^sub>t) ((env\<^sub>t, TApply # op # cd\<^sub>t) # sfs\<^sub>t))" by simp
-  moreover have "TS (v\<^sub>t # TLam env\<^sub>t' cd\<^sub>t' # vs\<^sub>t) ((env\<^sub>t, TApply # op # cd\<^sub>t) # sfs\<^sub>t) \<leadsto>\<^sub>t 
-    TS vs\<^sub>t ((v\<^sub>t # env\<^sub>t', cd\<^sub>t') # (env\<^sub>t, op # cd\<^sub>t) # sfs\<^sub>t)" by simp
-  ultimately have X: "iter (\<leadsto>\<^sub>t) (TS (v\<^sub>t # TLam env\<^sub>t' cd\<^sub>t' # vs\<^sub>t) 
-    (dsfs @ (env\<^sub>t, TApply # op # cd\<^sub>t) # sfs\<^sub>t)) (TS vs\<^sub>t ((v\<^sub>t # env\<^sub>t', cd\<^sub>t') # (env\<^sub>t, op # cd\<^sub>t) # sfs\<^sub>t))" 
+  from S have "iter (\<leadsto>\<^sub>e) (S\<^sub>e (v\<^sub>t # Lam\<^sub>e env\<^sub>t' cd\<^sub>t' # vs\<^sub>t) (dsfs @ (env\<^sub>t, Apply\<^sub>e # op # cd\<^sub>t) # sfs\<^sub>t)) 
+    (S\<^sub>e (v\<^sub>t # Lam\<^sub>e env\<^sub>t' cd\<^sub>t' # vs\<^sub>t) ((env\<^sub>t, Apply\<^sub>e # op # cd\<^sub>t) # sfs\<^sub>t))" by simp
+  moreover have "S\<^sub>e (v\<^sub>t # Lam\<^sub>e env\<^sub>t' cd\<^sub>t' # vs\<^sub>t) ((env\<^sub>t, Apply\<^sub>e # op # cd\<^sub>t) # sfs\<^sub>t) \<leadsto>\<^sub>e 
+    S\<^sub>e vs\<^sub>t ((v\<^sub>t # env\<^sub>t', cd\<^sub>t') # (env\<^sub>t, op # cd\<^sub>t) # sfs\<^sub>t)" by simp
+  ultimately have X: "iter (\<leadsto>\<^sub>e) (S\<^sub>e (v\<^sub>t # Lam\<^sub>e env\<^sub>t' cd\<^sub>t' # vs\<^sub>t) 
+    (dsfs @ (env\<^sub>t, Apply\<^sub>e # op # cd\<^sub>t) # sfs\<^sub>t)) (S\<^sub>e vs\<^sub>t ((v\<^sub>t # env\<^sub>t', cd\<^sub>t') # (env\<^sub>t, op # cd\<^sub>t) # sfs\<^sub>t))" 
       by simp
-  from evtco_apply S V have "full_block cd\<^sub>t' 0 = Some (Suc 0)" by simp
-  hence "live_frame (tco_val v\<^sub>t # map tco_val env\<^sub>t', tco_cd cd\<^sub>t', tco_r cd\<^sub>t')" 
-    by (induction cd\<^sub>t' rule: tco_cd.induct) (simp_all split: list.splits)
-  with S have "iter (\<leadsto>\<^sub>t\<^sub>c\<^sub>o) (TCOS (map tco_val vs\<^sub>t) ((tco_val v\<^sub>t # map tco_val env\<^sub>t', tco_cd cd\<^sub>t', 
-    tco_r cd\<^sub>t') # (map tco_val env\<^sub>t, tco_cd (op # cd\<^sub>t), tco_r (TApply # op # cd\<^sub>t)) # tco_stack sfs\<^sub>t)) 
-      (tco_state (TS vs\<^sub>t ((v\<^sub>t # env\<^sub>t', cd\<^sub>t') # (env\<^sub>t, op # cd\<^sub>t) # sfs\<^sub>t)))" by simp
+  from S have "iter (\<leadsto>\<^sub>e\<^sub>c\<^sub>o) (TCOS (map tco_val vs\<^sub>t) ((tco_val v\<^sub>t # map tco_val env\<^sub>t', tco_cd cd\<^sub>t', 
+    tco_r cd\<^sub>t') # (map tco_val env\<^sub>t, tco_cd (op # cd\<^sub>t), tco_r (Apply\<^sub>e # op # cd\<^sub>t)) # tco_stack sfs\<^sub>t)) 
+      (tco_state (S\<^sub>e vs\<^sub>t ((v\<^sub>t # env\<^sub>t', cd\<^sub>t') # (env\<^sub>t, op # cd\<^sub>t) # sfs\<^sub>t)))" by simp
   with S C V X show ?case by blast
 next
   case (evtco_return vs env sfs)
-  then obtain dsfs vs' env' sfs' where S: "\<Sigma>\<^sub>t = TS vs' (dsfs @ (env', []) # sfs') \<and> 
+  then obtain dsfs vs' env' sfs' where S: "\<Sigma>\<^sub>t = S\<^sub>e vs' (dsfs @ (env', []) # sfs') \<and> 
     vs = map tco_val vs' \<and> env = map tco_val env' \<and> list_all dead_frame dsfs \<and> sfs = tco_stack sfs'" 
       by blast
-  hence "iter (\<leadsto>\<^sub>t) (TS vs' (dsfs @ (env', []) # sfs')) (TS vs' ((env', []) # sfs'))" by simp
-  moreover have "iter (\<leadsto>\<^sub>t) (TS vs' ((env', []) # sfs')) (TS vs' sfs')" by (simp add: iter_one)
-  ultimately have X: "iter (\<leadsto>\<^sub>t) (TS vs' (dsfs @ (env', []) # sfs')) (TS vs' sfs')" by simp
-  from S have "iter (\<leadsto>\<^sub>t\<^sub>c\<^sub>o) (TCOS vs sfs) (tco_state (TS vs' sfs'))" by simp
+  hence "iter (\<leadsto>\<^sub>e) (S\<^sub>e vs' (dsfs @ (env', []) # sfs')) (S\<^sub>e vs' ((env', []) # sfs'))" by simp
+  moreover have "iter (\<leadsto>\<^sub>e) (S\<^sub>e vs' ((env', []) # sfs')) (S\<^sub>e vs' sfs')" by (simp add: iter_one)
+  ultimately have X: "iter (\<leadsto>\<^sub>e) (S\<^sub>e vs' (dsfs @ (env', []) # sfs')) (S\<^sub>e vs' sfs')" by simp
+  from S have "iter (\<leadsto>\<^sub>e\<^sub>c\<^sub>o) (TCOS vs sfs) (tco_state (S\<^sub>e vs' sfs'))" by simp
   with S X show ?case by blast
 next
   case (evtco_jump v env' cd' r' vs env sfs)
   then obtain dsfs v\<^sub>t vl vs\<^sub>t env\<^sub>t cd\<^sub>t sfs\<^sub>t where S: 
-    "\<Sigma>\<^sub>t = TS (v\<^sub>t # vl # vs\<^sub>t) (dsfs @ (env\<^sub>t, cd\<^sub>t) # sfs\<^sub>t) \<and> v = tco_val v\<^sub>t \<and> 
+    "\<Sigma>\<^sub>t = S\<^sub>e (v\<^sub>t # vl # vs\<^sub>t) (dsfs @ (env\<^sub>t, cd\<^sub>t) # sfs\<^sub>t) \<and> v = tco_val v\<^sub>t \<and> 
       TCOLam env' cd' r' = tco_val vl \<and> vs = map tco_val vs\<^sub>t \<and> env = map tco_val env\<^sub>t \<and> 
         [] = tco_cd cd\<^sub>t \<and> TCOJump = tco_r cd\<^sub>t \<and> list_all dead_frame dsfs \<and> 
           sfs = tco_stack sfs\<^sub>t" by blast
-  then obtain env\<^sub>t' cd\<^sub>t' where V: "vl = TLam env\<^sub>t' cd\<^sub>t' \<and> env' = map tco_val env\<^sub>t' \<and> 
+  then obtain env\<^sub>t' cd\<^sub>t' where V: "vl = Lam\<^sub>e env\<^sub>t' cd\<^sub>t' \<and> env' = map tco_val env\<^sub>t' \<and> 
     cd' = tco_cd cd\<^sub>t' \<and> r' = tco_r cd\<^sub>t'" by blast
-  from S have C: "cd\<^sub>t = [TApply]" by blast
-  with S have "iter (\<leadsto>\<^sub>t) (TS (v\<^sub>t # TLam env\<^sub>t' cd\<^sub>t' # vs\<^sub>t) (dsfs @ (env\<^sub>t, [TApply]) # sfs\<^sub>t)) 
-    (TS (v\<^sub>t # TLam env\<^sub>t' cd\<^sub>t' # vs\<^sub>t) ((env\<^sub>t, [TApply]) # sfs\<^sub>t))" by simp
-  moreover have "iter (\<leadsto>\<^sub>t) (TS (v\<^sub>t # TLam env\<^sub>t' cd\<^sub>t' # vs\<^sub>t) ((env\<^sub>t, [TApply]) # sfs\<^sub>t))
-    (TS vs\<^sub>t ((v\<^sub>t # env\<^sub>t', cd\<^sub>t') # (env\<^sub>t, []) # sfs\<^sub>t))" by (simp add: iter_one)
-  ultimately have X: "iter (\<leadsto>\<^sub>t) (TS (v\<^sub>t # TLam env\<^sub>t' cd\<^sub>t' # vs\<^sub>t) (dsfs @ (env\<^sub>t, [TApply]) # sfs\<^sub>t)) 
-    (TS vs\<^sub>t ((v\<^sub>t # env\<^sub>t', cd\<^sub>t') # (env\<^sub>t, []) # sfs\<^sub>t))" using iter_append by fastforce
-  have "iter (\<leadsto>\<^sub>t\<^sub>c\<^sub>o) (TCOS (map tco_val vs\<^sub>t) ((tco_val v\<^sub>t # map tco_val env\<^sub>t', tco_cd cd\<^sub>t', tco_r cd\<^sub>t') 
-    # tco_stack sfs\<^sub>t)) (tco_state (TS vs\<^sub>t ((v\<^sub>t # env\<^sub>t', cd\<^sub>t') # (env\<^sub>t, []) # sfs\<^sub>t)))" by simp
+  from S have C: "cd\<^sub>t = [Apply\<^sub>e]" by blast
+  with S have "iter (\<leadsto>\<^sub>e) (S\<^sub>e (v\<^sub>t # Lam\<^sub>e env\<^sub>t' cd\<^sub>t' # vs\<^sub>t) (dsfs @ (env\<^sub>t, [Apply\<^sub>e]) # sfs\<^sub>t)) 
+    (S\<^sub>e (v\<^sub>t # Lam\<^sub>e env\<^sub>t' cd\<^sub>t' # vs\<^sub>t) ((env\<^sub>t, [Apply\<^sub>e]) # sfs\<^sub>t))" by simp
+  moreover have "iter (\<leadsto>\<^sub>e) (S\<^sub>e (v\<^sub>t # Lam\<^sub>e env\<^sub>t' cd\<^sub>t' # vs\<^sub>t) ((env\<^sub>t, [Apply\<^sub>e]) # sfs\<^sub>t))
+    (S\<^sub>e vs\<^sub>t ((v\<^sub>t # env\<^sub>t', cd\<^sub>t') # (env\<^sub>t, []) # sfs\<^sub>t))" by (simp add: iter_one)
+  ultimately have X: "iter (\<leadsto>\<^sub>e) (S\<^sub>e (v\<^sub>t # Lam\<^sub>e env\<^sub>t' cd\<^sub>t' # vs\<^sub>t) (dsfs @ (env\<^sub>t, [Apply\<^sub>e]) # sfs\<^sub>t)) 
+    (S\<^sub>e vs\<^sub>t ((v\<^sub>t # env\<^sub>t', cd\<^sub>t') # (env\<^sub>t, []) # sfs\<^sub>t))" using iter_append by fastforce
+  have "iter (\<leadsto>\<^sub>e\<^sub>c\<^sub>o) (TCOS (map tco_val vs\<^sub>t) ((tco_val v\<^sub>t # map tco_val env\<^sub>t', tco_cd cd\<^sub>t', tco_r cd\<^sub>t') 
+    # tco_stack sfs\<^sub>t)) (tco_state (S\<^sub>e vs\<^sub>t ((v\<^sub>t # env\<^sub>t', cd\<^sub>t') # (env\<^sub>t, []) # sfs\<^sub>t)))" by simp
   with S V C X show ?case by blast
 qed
 
-theorem correcttco [simp]: "\<Sigma> \<leadsto>\<^sub>t \<Sigma>' \<Longrightarrow> iter (\<leadsto>\<^sub>t\<^sub>c\<^sub>o) (tco_state \<Sigma>) (tco_state \<Sigma>')"
-proof (induction \<Sigma> \<Sigma>' rule: evalt.induct)
-  case (evt_lookup env x v vs cd sfs)
+theorem correcttco [simp]: "\<Sigma> \<leadsto>\<^sub>e \<Sigma>' \<Longrightarrow> iter (\<leadsto>\<^sub>e\<^sub>c\<^sub>o) (tco_state \<Sigma>) (tco_state \<Sigma>')"
+proof (induction \<Sigma> \<Sigma>' rule: eval\<^sub>e.induct)
+  case (ev\<^sub>e_lookup env x v vs cd sfs)
   thus ?case 
   proof (cases cd)
     case Nil
-    have "TCOS (tco_val v # map tco_val vs) ((map tco_val env, [], TCOReturn) # tco_stack sfs) \<leadsto>\<^sub>t\<^sub>c\<^sub>o 
+    have "TCOS (tco_val v # map tco_val vs) ((map tco_val env, [], TCOReturn) # tco_stack sfs) \<leadsto>\<^sub>e\<^sub>c\<^sub>o 
       TCOS (tco_val v # map tco_val vs) (tco_stack sfs)" by (metis evtco_return)
-    hence "TCOS (tco_val v # map tco_val vs) ((map tco_val env, [], TCOReturn) # tco_stack sfs) \<leadsto>\<^sub>t\<^sub>c\<^sub>o 
-      tco_state (TS (v # vs) ((env, []) # sfs))" by simp
-    moreover from evt_lookup have "tco_state (TS vs ((env, [TLookup x]) # sfs)) \<leadsto>\<^sub>t\<^sub>c\<^sub>o
+    hence "TCOS (tco_val v # map tco_val vs) ((map tco_val env, [], TCOReturn) # tco_stack sfs) \<leadsto>\<^sub>e\<^sub>c\<^sub>o 
+      tco_state (S\<^sub>e (v # vs) ((env, []) # sfs))" by simp
+    moreover from ev\<^sub>e_lookup have "tco_state (S\<^sub>e vs ((env, [Lookup\<^sub>e x]) # sfs)) \<leadsto>\<^sub>e\<^sub>c\<^sub>o
       TCOS (tco_val v # map tco_val vs) ((map tco_val env, [], TCOReturn) # tco_stack sfs)" by simp
-    ultimately have "iter (\<leadsto>\<^sub>t\<^sub>c\<^sub>o) (tco_state (TS vs ((env, [TLookup x]) # sfs)))
-      (tco_state (TS (v # vs) ((env, []) # sfs)))" by (metis iter_refl iter_step)
+    ultimately have "iter (\<leadsto>\<^sub>e\<^sub>c\<^sub>o) (tco_state (S\<^sub>e vs ((env, [Lookup\<^sub>e x]) # sfs)))
+      (tco_state (S\<^sub>e (v # vs) ((env, []) # sfs)))" by (metis iter_refl iter_step)
     with Nil show ?thesis by simp
   next
     case (Cons op cd)
-    moreover from evt_lookup have "tco_state (TS vs ((env, TLookup x # op # cd) # sfs)) \<leadsto>\<^sub>t\<^sub>c\<^sub>o
-      tco_state (TS (v # vs) ((env, op # cd) # sfs))" by simp
+    moreover from ev\<^sub>e_lookup have "tco_state (S\<^sub>e vs ((env, Lookup\<^sub>e x # op # cd) # sfs)) \<leadsto>\<^sub>e\<^sub>c\<^sub>o
+      tco_state (S\<^sub>e (v # vs) ((env, op # cd) # sfs))" by simp
     ultimately show ?thesis by (metis iter_one)
   qed
 next
-  case (evt_pushcon vs env k cd sfs)
+  case (ev\<^sub>e_pushcon vs env k cd sfs)
   thus ?case 
   proof (cases cd)
     case Nil
-    have "TCOS (TCOConst k # map tco_val vs) ((map tco_val env, [], TCOReturn) # tco_stack sfs) \<leadsto>\<^sub>t\<^sub>c\<^sub>o 
+    have "TCOS (TCOConst k # map tco_val vs) ((map tco_val env, [], TCOReturn) # tco_stack sfs) \<leadsto>\<^sub>e\<^sub>c\<^sub>o 
         TCOS (TCOConst k # map tco_val vs) (tco_stack sfs)" by (metis evtco_return)
     hence "TCOS (TCOConst k # map tco_val vs) 
-      ((map tco_val env, [], TCOReturn) # tco_stack sfs) \<leadsto>\<^sub>t\<^sub>c\<^sub>o 
-        tco_state (TS (TConst k # vs) ((env, []) # sfs))" by simp
-    moreover have "tco_state (TS vs ((env, [TPushCon k]) # sfs)) \<leadsto>\<^sub>t\<^sub>c\<^sub>o
+      ((map tco_val env, [], TCOReturn) # tco_stack sfs) \<leadsto>\<^sub>e\<^sub>c\<^sub>o 
+        tco_state (S\<^sub>e (Const\<^sub>e k # vs) ((env, []) # sfs))" by simp
+    moreover have "tco_state (S\<^sub>e vs ((env, [PushCon\<^sub>e k]) # sfs)) \<leadsto>\<^sub>e\<^sub>c\<^sub>o
       TCOS (TCOConst k # map tco_val vs) 
         ((map tco_val env, [], TCOReturn) # tco_stack sfs)" by simp
-    ultimately have "iter (\<leadsto>\<^sub>t\<^sub>c\<^sub>o) (tco_state (TS vs ((env, [TPushCon k]) # sfs)))
-      (tco_state (TS (TConst k # vs) ((env, []) # sfs)))" by (metis iter_refl iter_step)
+    ultimately have "iter (\<leadsto>\<^sub>e\<^sub>c\<^sub>o) (tco_state (S\<^sub>e vs ((env, [PushCon\<^sub>e k]) # sfs)))
+      (tco_state (S\<^sub>e (Const\<^sub>e k # vs) ((env, []) # sfs)))" by (metis iter_refl iter_step)
     with Nil show ?thesis by simp
   next
     case (Cons op cd)
-    moreover have "tco_state (TS vs ((env, TPushCon k # op # cd) # sfs)) \<leadsto>\<^sub>t\<^sub>c\<^sub>o
-      tco_state (TS (TConst k # vs) ((env, op # cd) # sfs))" by simp
+    moreover have "tco_state (S\<^sub>e vs ((env, PushCon\<^sub>e k # op # cd) # sfs)) \<leadsto>\<^sub>e\<^sub>c\<^sub>o
+      tco_state (S\<^sub>e (Const\<^sub>e k # vs) ((env, op # cd) # sfs))" by simp
     ultimately show ?thesis by (metis iter_one)
   qed
 next
-  case (evt_pushlam vs env cd' cd sfs)
+  case (ev\<^sub>e_pushlam vs env cd' cd sfs)
   thus ?case 
   proof (cases cd)
     case Nil
     have "TCOS (map tco_val vs) ((map tco_val env, 
-      [TCOPushLam (tco_cd cd') (tco_r cd')], TCOReturn) # tco_stack sfs) \<leadsto>\<^sub>t\<^sub>c\<^sub>o  
+      [TCOPushLam (tco_cd cd') (tco_r cd')], TCOReturn) # tco_stack sfs) \<leadsto>\<^sub>e\<^sub>c\<^sub>o  
         TCOS (TCOLam (map tco_val env) (tco_cd cd') (tco_r cd') # map tco_val vs) 
           ((map tco_val env, [], TCOReturn) # tco_stack sfs)" by (metis evtco_pushlam)
-    hence X: "tco_state (TS vs ((env, [TPushLam cd']) # sfs)) \<leadsto>\<^sub>t\<^sub>c\<^sub>o
+    hence X: "tco_state (S\<^sub>e vs ((env, [PushLam\<^sub>e cd']) # sfs)) \<leadsto>\<^sub>e\<^sub>c\<^sub>o
       TCOS (TCOLam (map tco_val env) (tco_cd cd') (tco_r cd') # map tco_val vs) 
         ((map tco_val env, [], TCOReturn) # tco_stack sfs)" by simp
     have "TCOS (TCOLam (map tco_val env) (tco_cd cd') (tco_r cd') # 
-      map tco_val vs) ((map tco_val env, [], TCOReturn) # tco_stack sfs) \<leadsto>\<^sub>t\<^sub>c\<^sub>o
+      map tco_val vs) ((map tco_val env, [], TCOReturn) # tco_stack sfs) \<leadsto>\<^sub>e\<^sub>c\<^sub>o
         TCOS (TCOLam (map tco_val env) (tco_cd cd') (tco_r cd') # map tco_val vs) (tco_stack sfs)" 
           by (metis evtco_return)
     hence "TCOS (TCOLam (map tco_val env) (tco_cd cd') (tco_r cd') # 
-      map tco_val vs) ((map tco_val env, [], TCOReturn) # tco_stack sfs) \<leadsto>\<^sub>t\<^sub>c\<^sub>o
-        tco_state (TS (TLam env cd' # vs) ((env, []) # sfs))" by simp
-    with X have "iter (\<leadsto>\<^sub>t\<^sub>c\<^sub>o) (tco_state (TS vs ((env, [TPushLam cd']) # sfs)))
-      (tco_state (TS (TLam env cd' # vs) ((env, []) # sfs)))" by (metis iter_refl iter_step)
+      map tco_val vs) ((map tco_val env, [], TCOReturn) # tco_stack sfs) \<leadsto>\<^sub>e\<^sub>c\<^sub>o
+        tco_state (S\<^sub>e (Lam\<^sub>e env cd' # vs) ((env, []) # sfs))" by simp
+    with X have "iter (\<leadsto>\<^sub>e\<^sub>c\<^sub>o) (tco_state (S\<^sub>e vs ((env, [PushLam\<^sub>e cd']) # sfs)))
+      (tco_state (S\<^sub>e (Lam\<^sub>e env cd' # vs) ((env, []) # sfs)))" by (metis iter_refl iter_step)
     with Nil show ?thesis by simp
   next
     case (Cons op cd)
     have "TCOS (map tco_val vs) ((map tco_val env, TCOPushLam (tco_cd cd') (tco_r cd') # 
-      tco_cd (op # cd), tco_r (op # cd)) # tco_stack sfs) \<leadsto>\<^sub>t\<^sub>c\<^sub>o
+      tco_cd (op # cd), tco_r (op # cd)) # tco_stack sfs) \<leadsto>\<^sub>e\<^sub>c\<^sub>o
         TCOS (TCOLam (map tco_val env) (tco_cd cd') (tco_r cd') # map tco_val vs) 
           ((map tco_val env, tco_cd (op # cd), tco_r (op # cd)) # tco_stack sfs)" 
       by (metis evtco_pushlam)
-    hence "tco_state (TS vs ((env, TPushLam cd' # op # cd) # sfs)) \<leadsto>\<^sub>t\<^sub>c\<^sub>o
-      tco_state (TS (TLam env cd' # vs) ((env, op # cd) # sfs))" by simp
+    hence "tco_state (S\<^sub>e vs ((env, PushLam\<^sub>e cd' # op # cd) # sfs)) \<leadsto>\<^sub>e\<^sub>c\<^sub>o
+      tco_state (S\<^sub>e (Lam\<^sub>e env cd' # vs) ((env, op # cd) # sfs))" by simp
     with Cons show ?thesis by (metis iter_one)
   qed
 next
-  case (evt_apply v env' cd' vs env cd sfs)
+  case (ev\<^sub>e_apply v env' cd' vs env cd sfs)
   thus ?case 
   proof (cases cd)
     case Nil note CD = Nil
@@ -347,29 +344,29 @@ next
     proof (cases cd')
       case Nil
       have "TCOS (map tco_val vs) ((tco_val v # map tco_val env', [], TCOReturn) # tco_stack sfs) 
-        \<leadsto>\<^sub>t\<^sub>c\<^sub>o TCOS (map tco_val vs) (tco_stack sfs)" by (metis evtco_return)
+        \<leadsto>\<^sub>e\<^sub>c\<^sub>o TCOS (map tco_val vs) (tco_stack sfs)" by (metis evtco_return)
       hence "TCOS (map tco_val vs) ((tco_val v # map tco_val env', [], TCOReturn) # tco_stack sfs) 
-        \<leadsto>\<^sub>t\<^sub>c\<^sub>o tco_state (TS vs ((v # env', []) # (env, []) # sfs))" by simp
-      hence X: "iter (\<leadsto>\<^sub>t\<^sub>c\<^sub>o) (TCOS (map tco_val vs) ((tco_val v # map tco_val env', [], TCOReturn) # 
-        tco_stack sfs)) (tco_state (TS vs ((v # env', []) # (env, []) # sfs)))" by (metis iter_one)
+        \<leadsto>\<^sub>e\<^sub>c\<^sub>o tco_state (S\<^sub>e vs ((v # env', []) # (env, []) # sfs))" by simp
+      hence X: "iter (\<leadsto>\<^sub>e\<^sub>c\<^sub>o) (TCOS (map tco_val vs) ((tco_val v # map tco_val env', [], TCOReturn) # 
+        tco_stack sfs)) (tco_state (S\<^sub>e vs ((v # env', []) # (env, []) # sfs)))" by (metis iter_one)
       have "TCOS (tco_val v # TCOLam (map tco_val env') [] TCOReturn # 
-        map tco_val vs) ((map tco_val env, [], TCOJump) # tco_stack sfs) \<leadsto>\<^sub>t\<^sub>c\<^sub>o
+        map tco_val vs) ((map tco_val env, [], TCOJump) # tco_stack sfs) \<leadsto>\<^sub>e\<^sub>c\<^sub>o
           TCOS (map tco_val vs) ((tco_val v # map tco_val env', [], TCOReturn) # 
             tco_stack sfs)" by (metis evtco_jump)
-      hence "tco_state (TS (v # TLam env' [] # vs) ((env, [TApply]) # sfs)) \<leadsto>\<^sub>t\<^sub>c\<^sub>o
+      hence "tco_state (S\<^sub>e (v # Lam\<^sub>e env' [] # vs) ((env, [Apply\<^sub>e]) # sfs)) \<leadsto>\<^sub>e\<^sub>c\<^sub>o
         TCOS (map tco_val vs) ((tco_val v # map tco_val env', [], TCOReturn) # tco_stack sfs)" 
           by simp
-      with X have "iter (\<leadsto>\<^sub>t\<^sub>c\<^sub>o) (tco_state (TS (v # TLam env' [] # vs) ((env, [TApply]) # sfs)))
-        (tco_state (TS vs ((v # env', []) # (env, []) # sfs)))" using iter_step by fast
+      with X have "iter (\<leadsto>\<^sub>e\<^sub>c\<^sub>o) (tco_state (S\<^sub>e (v # Lam\<^sub>e env' [] # vs) ((env, [Apply\<^sub>e]) # sfs)))
+        (tco_state (S\<^sub>e vs ((v # env', []) # (env, []) # sfs)))" using iter_step by fast
       with CD Nil show ?thesis by simp
     next
       case (Cons op' cd'')
       have "TCOS (tco_val v # TCOLam (map tco_val env') (tco_cd (op' # cd'')) (tco_r (op' # cd'')) # 
-        map tco_val vs) ((map tco_val env, [], TCOJump) # tco_stack sfs) \<leadsto>\<^sub>t\<^sub>c\<^sub>o
+        map tco_val vs) ((map tco_val env, [], TCOJump) # tco_stack sfs) \<leadsto>\<^sub>e\<^sub>c\<^sub>o
           TCOS (map tco_val vs) ((tco_val v # map tco_val env', tco_cd (op' # cd''), 
             tco_r (op' # cd'')) # tco_stack sfs)"  by (metis evtco_jump)
-      hence "tco_state (TS (v # TLam env' (op' # cd'') # vs) ((env, [TApply]) # sfs)) \<leadsto>\<^sub>t\<^sub>c\<^sub>o
-        tco_state (TS vs ((v # env', op' # cd'') # (env, []) # sfs))" by simp
+      hence "tco_state (S\<^sub>e (v # Lam\<^sub>e env' (op' # cd'') # vs) ((env, [Apply\<^sub>e]) # sfs)) \<leadsto>\<^sub>e\<^sub>c\<^sub>o
+        tco_state (S\<^sub>e vs ((v # env', op' # cd'') # (env, []) # sfs))" by simp
       with Nil Cons show ?thesis by (metis iter_one)
     qed
   next
@@ -378,34 +375,34 @@ next
     proof (cases cd')
       case Nil
       have "TCOS (map tco_val vs) ((tco_val v # map tco_val env', [], TCOReturn) # 
-        (map tco_val env, tco_cd (op # cd), tco_r (op # cd)) # tco_stack sfs) \<leadsto>\<^sub>t\<^sub>c\<^sub>o
+        (map tco_val env, tco_cd (op # cd), tco_r (op # cd)) # tco_stack sfs) \<leadsto>\<^sub>e\<^sub>c\<^sub>o
           TCOS (map tco_val vs) ((map tco_val env, tco_cd (op # cd), 
             tco_r (op # cd)) # tco_stack sfs)" by (metis evtco_return)
       hence "TCOS (map tco_val vs) ((tco_val v # map tco_val env', [], TCOReturn) # 
-        (map tco_val env, tco_cd (op # cd), tco_r (op # cd)) # tco_stack sfs) \<leadsto>\<^sub>t\<^sub>c\<^sub>o
-            tco_state (TS vs ((v # env', []) # (env, op # cd) # sfs))" by simp
-      hence X: "iter (\<leadsto>\<^sub>t\<^sub>c\<^sub>o) (TCOS (map tco_val vs) ((tco_val v # map tco_val env', [], TCOReturn) # 
+        (map tco_val env, tco_cd (op # cd), tco_r (op # cd)) # tco_stack sfs) \<leadsto>\<^sub>e\<^sub>c\<^sub>o
+            tco_state (S\<^sub>e vs ((v # env', []) # (env, op # cd) # sfs))" by simp
+      hence X: "iter (\<leadsto>\<^sub>e\<^sub>c\<^sub>o) (TCOS (map tco_val vs) ((tco_val v # map tco_val env', [], TCOReturn) # 
         (map tco_val env, tco_cd (op # cd), tco_r (op # cd)) # tco_stack sfs)) 
-          (tco_state (TS vs ((v # env', []) # (env, op # cd) # sfs)))" by (metis iter_one)
-      have "tco_state (TS (v # TLam env' [] # vs) ((env, TApply # op # cd) # sfs)) \<leadsto>\<^sub>t\<^sub>c\<^sub>o
+          (tco_state (S\<^sub>e vs ((v # env', []) # (env, op # cd) # sfs)))" by (metis iter_one)
+      have "tco_state (S\<^sub>e (v # Lam\<^sub>e env' [] # vs) ((env, Apply\<^sub>e # op # cd) # sfs)) \<leadsto>\<^sub>e\<^sub>c\<^sub>o
         TCOS (map tco_val vs) ((tco_val v # map tco_val env', [], TCOReturn) # 
           (map tco_val env, tco_cd (op # cd), tco_r (op # cd)) # tco_stack sfs)" by simp
-      with X have "iter (\<leadsto>\<^sub>t\<^sub>c\<^sub>o) (tco_state (TS (v # TLam env' [] # vs) 
-        ((env, TApply # op # cd) # sfs)))
-          (tco_state (TS vs ((v # env', []) # (env, op # cd) # sfs)))" 
+      with X have "iter (\<leadsto>\<^sub>e\<^sub>c\<^sub>o) (tco_state (S\<^sub>e (v # Lam\<^sub>e env' [] # vs) 
+        ((env, Apply\<^sub>e # op # cd) # sfs)))
+          (tco_state (S\<^sub>e vs ((v # env', []) # (env, op # cd) # sfs)))" 
         using iter_step by fast
       with Cons Nil show ?thesis by simp
     next
       case (Cons op' cd')
-      have "tco_state (TS (v # TLam env' (op' # cd') # vs) 
-        ((env, TApply # op # cd) # sfs)) \<leadsto>\<^sub>t\<^sub>c\<^sub>o
-          tco_state (TS vs ((v # env', (op' # cd')) # (env, op # cd) # sfs))" by simp
+      have "tco_state (S\<^sub>e (v # Lam\<^sub>e env' (op' # cd') # vs) 
+        ((env, Apply\<^sub>e # op # cd) # sfs)) \<leadsto>\<^sub>e\<^sub>c\<^sub>o
+          tco_state (S\<^sub>e vs ((v # env', (op' # cd')) # (env, op # cd) # sfs))" by simp
       with CD Cons show ?thesis by (metis iter_one)
     qed
   qed
 qed simp_all
 
-lemma iter_tco_eval [simp]: "iter (\<leadsto>\<^sub>t) \<Sigma> \<Sigma>' \<Longrightarrow> iter (\<leadsto>\<^sub>t\<^sub>c\<^sub>o) (tco_state \<Sigma>) (tco_state \<Sigma>')"
+lemma iter_tco_eval [simp]: "iter (\<leadsto>\<^sub>e) \<Sigma> \<Sigma>' \<Longrightarrow> iter (\<leadsto>\<^sub>e\<^sub>c\<^sub>o) (tco_state \<Sigma>) (tco_state \<Sigma>')"
   by (induction \<Sigma> \<Sigma>' rule: iter.induct) (simp, metis iter_append correcttco)
 
 end
